core/AssertionNotations.v
@@ -1,0 +1,45 @@
+Require Import Coq.Strings.String.
+Require Import Poulet4.Typed.
+Require Import Poulet4.Syntax.
+Require Import Poulet4.Semantics.
+Require Import Poulet4.Value.
+Require Import ProD3.core.Coqlib.
+Require Import ProD3.core.Hoare.
+Require Import ProD3.core.SvalRefine.
+Require Import ProD3.core.AssertionLang.
+Open Scope type_scope.
+
+Section AssertionNotations.
+
+Context {tags_t: Type} {tags_t_inhabitant : Inhabitant tags_t}.
+Notation Val := (@ValueBase bool).
+Notation Sval := (@ValueBase (option bool)).
+Notation Lval := ValueLvalue.
+
+Notation ident := (string).
+Notation path := (list ident).
+Notation P4Int := (P4Int.t tags_t).
+Notation P4String := (P4String.t tags_t).
+Notation P4Type := (@P4Type tags_t).
+Notation mem := Semantics.mem.
+
+Context `{@Target tags_t (@Expression tags_t)}.
+
+Definition EXT : ext_assertion -> ext_assertion :=
+  id.
+
+Definition MEM (a_mem : mem_assertion) (a_ext : ext_assertion) : Hoare.assertion :=
+  fun '(m, es) => mem_denote a_mem m /\ ext_denote a_ext es.
+
+Definition ARG (a_arg : list Sval) (a : Hoare.assertion) : Hoare.arg_assertion :=
+  fun args st => arg_denote a_arg args /\ a st.
+
+Definition RET (a_ret : Sval) (a : Hoare.assertion) : Hoare.ret_assertion :=
+  fun retv st => (forall sv', val_to_sval retv sv' -> ret_denote a_ret sv') /\ a st.
+
+Definition ARG_RET (a_arg : list Sval) (a_ret : Sval) (a : Hoare.assertion) : Hoare.arg_ret_assertion :=
+  fun args retv st => arg_denote a_arg args
+    /\ (forall sv', val_to_sval retv sv' -> ret_denote a_ret sv')
+    /\ a st.
+
+End AssertionNotations.
